examples/Isa.v
@@ -1,0 +1,67 @@
+Require Import Bool String List.
+Require Import Lib.CommonTactics Lib.Word.
+Require Import Lts.Syntax Lts.Notations.
+Require Import Ex.SC.
+
+(* Subset of RV32I instructions *)
+Section RV32ISubset.
+
+  Definition rv32iAddrSize := 32.
+  Definition rv32iLgDataBytes := 4.
+  Definition rv32iOpIdx := 7. (* always inst[6-0] *)
+  Definition rv32iRfIdx := 5. (* 2^5 = 32 general purpose registers, x0 is hardcoded though *)
+
+  Definition rv32iLd := WO~0~0~0~0~0~1~1.
+  Definition rv32iSt := WO~0~1~0~0~0~1~1.
+  Definition rv32iOp := WO~0~1~1~0~0~1~1. (* Register-Register operations *)
+
+  Definition getRs1ValueE {ty}
+             (s : StateT rv32iLgDataBytes rv32iRfIdx ty)
+             (inst : fullType ty (SyntaxKind (Bit rv32iAddrSize))) :=
+    (#s @[UniBit (ConstExtract 12 5 _) #inst])%kami_expr.
+  Definition getRs2ValueE {ty}
+             (s : StateT rv32iLgDataBytes rv32iRfIdx ty)
+             (inst : fullType ty (SyntaxKind (Bit rv32iAddrSize))) :=
+    (#s @[UniBit (ConstExtract 7 5 _) #inst])%kami_expr.
+  Definition getLdBaseE {ty}
+             (inst : fullType ty (SyntaxKind (Bit rv32iAddrSize))) :=
+    (UniBit (ZeroExtendTrunc _ rv32iAddrSize) (UniBit (TruncLsb 12 _) #inst))%kami_expr.
+  Definition getStBaseE {ty}
+             (inst : fullType ty (SyntaxKind (Bit rv32iAddrSize))) :=
+    (UniBit (ZeroExtendTrunc _ rv32iAddrSize) (UniBit (TruncLsb 7 _) #inst))%kami_expr.
+
+  Definition rv32iDecode: DecT rv32iOpIdx rv32iAddrSize rv32iLgDataBytes rv32iRfIdx.
+    unfold DecT; intros ty s inst.
+    refine (IF ((UniBit (Trunc (rv32iAddrSize - rv32iOpIdx) _) #inst)
+                == (Const _ rv32iLd)) then _ else _)%kami_expr.
+    - (* load case *)
+      exact (STRUCT { "opcode" ::= UniBit (Trunc (rv32iAddrSize - rv32iOpIdx) _) #inst;
+                      "reg" ::= UniBit (ConstExtract 20 5 _) #inst;
+                      "addr" ::= (getRs1ValueE s inst + getLdBaseE inst);
+                      "value" ::= $$Default })%kami_expr.
+    - refine (IF ((UniBit (Trunc (rv32iAddrSize - rv32iOpIdx) _) #inst)
+                  == (Const _ rv32iSt)) then _ else _)%kami_expr.
+      + (* store case *)
+        exact (STRUCT { "opcode" ::= (UniBit (Trunc (rv32iAddrSize - rv32iOpIdx) _) #inst);
+                        "reg" ::= $$Default;
+                        "addr" ::= (getRs1ValueE s inst + getStBaseE inst);
+                        "value" ::= getRs2ValueE s inst })%kami_expr.
+      + (* non-memory operations *)
+        exact (STRUCT { "opcode" ::= (UniBit (Trunc (rv32iAddrSize - rv32iOpIdx) _) #inst);
+                        "reg" ::= $$Default;
+                        "addr" ::= $$Default;
+                        "value" ::= $$Default })%kami_expr.
+  Defined.
+
+  Definition rv32iExecState: ExecStateT rv32iOpIdx rv32iAddrSize rv32iLgDataBytes rv32iRfIdx.
+    unfold ExecStateT; intros ty s pc inst.
+    exact (#s)%kami_expr. (* TODO: implement *)
+  Defined.
+
+  Definition rv32iExecNextPc: ExecNextPcT rv32iOpIdx rv32iAddrSize rv32iLgDataBytes rv32iRfIdx.
+    unfold ExecStateT; intros ty s pc inst.
+    exact (#pc + $4)%kami_expr.
+  Defined.
+
+End RV32ISubset.
+
